generalise Var_map, SimAsm_Exp, SimAsm.
uses new expression context, extending state and adding
a local variable names set.

SimAsm/SimAsm_Exp.thy
@@ -1,5 +1,5 @@
 theory SimAsm_Exp
-  imports SimAsm_State Var_map
+  imports State2 Var_map
 begin
 
 context expression
@@ -13,17 +13,17 @@ fun st_ev\<^sub>E
 
 
 text \<open>Evaluate a boolean expression given a state\<close>
-fun st_ev\<^sub>B :: "('v,'g,'r,'a) state \<Rightarrow> ('v,'g,'r) bexp \<Rightarrow> bool"
-  where  "st_ev\<^sub>B m r = ev\<^sub>B (lookupSome m) r" 
+fun st_ev\<^sub>B :: "'s \<Rightarrow> ('r,'v) bexp \<Rightarrow> bool"
+  where  "st_ev\<^sub>B m r = ev\<^sub>B (st m) r" 
 
 
 text \<open>Operation Behaviour\<close>
 
-fun st_beh\<^sub>i :: "('v,'g,'r) op \<Rightarrow> ('v,'g,'r,'a) state rel"
+fun st_beh\<^sub>i :: "('r,'v) op \<Rightarrow> 's rel"
   where
-    "st_beh\<^sub>i (assign a e) = {(s,s'). s' = s (a :=\<^sub>s (st_ev\<^sub>E (s) e))}" | 
+    "st_beh\<^sub>i (assign a e) = {(s,s'). s' =  s(a :=\<^sub>u (st_ev\<^sub>E (s) e))}" | 
     "st_beh\<^sub>i (cmp b) = {(s,s'). s = s' \<and> st_ev\<^sub>B s b}" |
-    "st_beh\<^sub>i (leak Cache e) = {(s,s'). s' = s (Cache :=\<^sub>b (st_ev\<^sub>E (s) e))}" | 
+    "st_beh\<^sub>i (leak Cache e) = {(s,s'). s' =  s(Cache :=\<^sub>u (st_ev\<^sub>E (s) e))}" | 
     "st_beh\<^sub>i _ = Id"
  
 
@@ -31,51 +31,43 @@ subsection \<open>Expression\<close>
 
 
 lemma st_ev_subst\<^sub>E [simp]:
-  "st_ev\<^sub>E m (subst\<^sub>E e r f) = st_ev\<^sub>E (m(r :=\<^sub>s (st_ev\<^sub>E m f))) e"
+  "st_ev\<^sub>E m (subst\<^sub>E e r f) = st_ev\<^sub>E (m(r :=\<^sub>u (st_ev\<^sub>E m f))) e"
 proof (induct e)
   case (Var x)
   then show ?case 
-  proof(cases "x=r")
-    case True
-    then show ?thesis by simp
-  next
-    case False
-    then show ?thesis using st_upd_def fun_upd_def ev\<^sub>E.simps(1) apply simp 
-      by (smt (verit) select_convs(3) st_upd_def surjective update_convs(1))
-  qed
+  by (cases "x=r") simp_all
 next
   case (Val x)
   then show ?case by simp
 next
   case (Exp fn rs)
-  hence [simp]: "map (st_ev\<^sub>E m \<circ> (\<lambda>x. subst\<^sub>E x r f)) rs = map (st_ev\<^sub>E (m(r :=\<^sub>s st_ev\<^sub>E m f))) rs" by auto
+  hence [simp]: "map (st_ev\<^sub>E m \<circ> (\<lambda>x. subst\<^sub>E x r f)) rs = map (st_ev\<^sub>E (m(r :=\<^sub>u st_ev\<^sub>E m f))) rs" by auto
   then show ?case  using ev\<^sub>E.simps(3) map_map subst\<^sub>E.simps(2) 
-  by (metis (no_types, lifting) map_eq_conv st_ev\<^sub>E.simps)
+  by (smt (verit, best) expression.ev_subst\<^sub>E' expression.st_ev\<^sub>E.simps expression_axioms state.st_upd_map state_axioms)
 qed                          
 
 
 lemma st_ev_nop\<^sub>E [simp]:
-  "r \<notin> deps\<^sub>E e \<Longrightarrow> st_ev\<^sub>E (m(r :=\<^sub>s f)) e = st_ev\<^sub>E m e"
+  "r \<notin> deps\<^sub>E e \<Longrightarrow> st_ev\<^sub>E (m(r :=\<^sub>u f)) e = st_ev\<^sub>E m e"
 proof (induct e)
   case (Var x)
   then show ?case using Var
   proof(cases "x=r")
     case True
     hence "r \<in> deps\<^sub>E (Var x)" using deps\<^sub>E.simps(1) by simp
-    then show ?thesis using st_upd_def Var by simp
+    then show ?thesis using Var by simp
   next
     case False
-    then show ?thesis using st_upd_def fun_upd_def ev\<^sub>E.simps(1) apply simp 
-      by (smt (verit) select_convs(3) st_upd_def surjective update_convs(1))
+    then show ?thesis using fun_upd_def ev\<^sub>E.simps(1) by simp 
   qed
 next
   case (Val x)
   then show ?case by simp
 next
   case (Exp fn rs)
-  hence [simp]: "map (st_ev\<^sub>E (m(r :=\<^sub>s f))) rs = map (st_ev\<^sub>E m) rs" by auto
-  then show ?case using ev\<^sub>E.simps(3) st_ev\<^sub>E.simps 
-    by (metis (mono_tags, lifting) map_eq_conv)
+  hence [simp]: "map (st_ev\<^sub>E (m(r :=\<^sub>u f))) rs = map (st_ev\<^sub>E m) rs" by auto
+  then show ?case using st_ev\<^sub>E.simps 
+    by (metis Exp.prems ev_nop\<^sub>E' st_upd_map)
 qed 
 
 term st
@@ -84,12 +76,12 @@ lemma deps_st_ev\<^sub>E [intro]:
   "(\<forall>x \<in> deps\<^sub>E e. st m x = st m' x) \<Longrightarrow> st_ev\<^sub>E m e = st_ev\<^sub>E m' e"
 proof (induct e)
   case (Var x)
-  then show ?case using equality st_ev\<^sub>E.simps deps\<^sub>E.simps(1) ev\<^sub>E.simps(1) 
+  then show ?case using st_ev\<^sub>E.simps deps\<^sub>E.simps(1) ev\<^sub>E.simps(1) 
   proof -
     have a0:"deps\<^sub>E (Var x) ={x}" by simp
     then have a1:"st m x = st m' x" using Var by simp
-    then have a2:"lookupSome m x = lookupSome m' x" using Var lookupSome.simps[of m x] 
-           lookupSome.simps[of m' x] sorry
+    (* then have a2:"lookupSome m x = lookupSome m' x" using Var lookupSome.simps[of m x]  *)
+           (* lookupSome.simps[of m' x] sorry *)
     then show ?thesis       using st_ev\<^sub>E.simps deps\<^sub>E.simps(1) ev\<^sub>E.simps(1) Var by simp
   qed
 next
@@ -103,63 +95,34 @@ next
 qed 
 
 
-lemma deps_st_ev\<^sub>E'' [intro]:
-  "\<forall>x \<in> deps\<^sub>E e . lookupSome s x = lookupSome s' x \<Longrightarrow> st_ev\<^sub>E s e = st_ev\<^sub>E s' e"
-proof (induct e)
-  case (Var x) 
-  show ?case using deps\<^sub>E.simps(1) st_ev\<^sub>E.simps(1) lookupSome.simps st_ev\<^sub>E.simps(1) using Var by simp
-  next
-  case (Val x)
-  then show ?case by auto
-next
-  case (Exp fn rs)
-  hence [simp]: "map (st_ev\<^sub>E s) rs = map (st_ev\<^sub>E s') rs" by (induct rs) auto
-  show ?case using st_ev\<^sub>E.simps by (metis (mono_tags, lifting) Exp.prems deps_ev\<^sub>E)
-qed
-
-
 lemma local_st_ev\<^sub>E [intro]:
-  "deps\<^sub>E e \<subseteq> locals \<Longrightarrow> rg m = rg m' \<Longrightarrow> st_ev\<^sub>E m e = st_ev\<^sub>E m' e"
-  apply (intro deps_st_ev\<^sub>E ballI, case_tac x) 
-  using rg_def apply simp
-  by blast  
-
+  "deps\<^sub>E e \<subseteq> locals \<Longrightarrow> (\<forall>v \<in> locals. st m v = st m' v) \<Longrightarrow> st_ev\<^sub>E m e = st_ev\<^sub>E m' e"
+  by auto
 
 lemma st_ev_aux\<^sub>E [simp]:
   "st_ev\<^sub>E (m(aux: f)) g = st_ev\<^sub>E m g"
-proof (induct g)
-  case (Var x)
-  then show ?case apply simp 
-    by (metis aux_upd_def select_convs(3) surjective update_convs(4))
-next
-  case (Val x)
-  then show ?case by simp 
-next
-  case (Exp x1a x2a)
-  then show ?case apply simp by (metis (mono_tags, lifting) map_eq_conv)
-qed
-
+by (induct g) (simp, simp, fastforce)
 
 subsection \<open>Boolean Expression\<close>
 
 lemma st_ev_subst\<^sub>B [simp]:
-  "st_ev\<^sub>B m (subst\<^sub>B b r e) = st_ev\<^sub>B (m(r :=\<^sub>s (st_ev\<^sub>E m e))) b"
+  "st_ev\<^sub>B m (subst\<^sub>B b r e) = st_ev\<^sub>B (m(r :=\<^sub>u (st_ev\<^sub>E m e))) b"
 proof (induct b)
   case (Exp\<^sub>B fn rs)
-  have [simp]: "map (st_ev\<^sub>E m \<circ> (\<lambda>x. subst\<^sub>E x r e)) rs = map (st_ev\<^sub>E (m(r :=\<^sub>s st_ev\<^sub>E m e))) rs"
-    using fun_upd_def apply simp sorry    
-  show ?case sorry
+  have [simp]: "map (st_ev\<^sub>E m \<circ> (\<lambda>x. subst\<^sub>E x r e)) rs = map (st_ev\<^sub>E (m(r :=\<^sub>u st_ev\<^sub>E m e))) rs"
+    using fun_upd_def by auto   
+  thus ?case by (metis ev_subst\<^sub>B st_ev\<^sub>B.elims(1) st_ev\<^sub>E.simps st_upd_map)
 qed simp
 
 
 
 lemma st_ev_nop\<^sub>B [simp]:
-  "r \<notin> deps\<^sub>B b \<Longrightarrow> st_ev\<^sub>B (m(r :=\<^sub>s f)) b = st_ev\<^sub>B m b"
+  "r \<notin> deps\<^sub>B b \<Longrightarrow> st_ev\<^sub>B (m(r :=\<^sub>u f)) b = st_ev\<^sub>B m b"
 proof (induct b)
   case (Exp\<^sub>B fn rs)
-  hence [simp]: "map (st_ev\<^sub>E (m(r :=\<^sub>s f))) rs = map (st_ev\<^sub>E m) rs"
+  hence [simp]: "map (st_ev\<^sub>E (m(r :=\<^sub>u f))) rs = map (st_ev\<^sub>E m) rs"
     using st_ev_nop\<^sub>E[of r _ m f] by (auto simp: fun_upd_def) 
-  show ?case sorry
+  then show ?case by (metis Exp\<^sub>B ev_nop\<^sub>B st_ev\<^sub>B.elims(1) st_upd_map)
 qed simp
 
 
@@ -167,8 +130,8 @@ lemma deps_st_ev\<^sub>B [intro]:
   "\<forall>x \<in> deps\<^sub>B e. st m x = st m' x \<Longrightarrow> st_ev\<^sub>B m e = st_ev\<^sub>B m' e"
 proof (induct e)
   case (Exp\<^sub>B fn rs)
-  hence [simp]: "map (st_ev\<^sub>E m) rs = map (st_ev\<^sub>E m') rs" sorry (* by (induct rs) auto *)
-  show ?case sorry
+  hence [simp]: "map (st_ev\<^sub>E m) rs = map (st_ev\<^sub>E m') rs" by (induct rs) auto
+  then show ?case by (metis (mono_tags, lifting) ev\<^sub>B.simps(2) map_eq_conv st_ev\<^sub>B.elims(1) st_ev\<^sub>E.elims)
 qed auto
 
 
@@ -179,12 +142,13 @@ proof (induct g)
   then show ?case by simp
 next
   case (Exp\<^sub>B x1a x2)
-  then show ?case using st_ev\<^sub>B.simps st_ev_aux\<^sub>E map_eq_conv sorry
+  then show ?case using st_ev\<^sub>B.simps st_ev_aux\<^sub>E map_eq_conv aux_upd_st by presburger
 qed
 
 
 subsection \<open>Update lemmas\<close>
 
+(*
 definition upd                   (* use if f is a total fun: 'a \<Rightarrow> 'v *)
   where "upd S f m \<equiv> m\<lparr>st := \<lambda>x. if x \<in> S then Some (f x) else st m x\<rparr>"
 
@@ -224,36 +188,34 @@ lemma upd_init [simp]:
   "state_rec.initState (upd V f m) = state_rec.initState m"
   by (auto simp: upd_def)
 
+*)
 
-
-
-thm state_rec.equality
 
 (* if \<Gamma> is in aux then this will include equality of \<Gamma> mapping *)
-lemma st_upd_eq [intro]:
-  "state_rec.more m = state_rec.more m' \<Longrightarrow> 
-              state_rec.cap m = state_rec.cap m' \<Longrightarrow>
-                 initState m = initState m' \<Longrightarrow>
-                    \<forall>x. x \<noteq> y \<longrightarrow> st m x = st m' x \<Longrightarrow> m(y :=\<^sub>s e) = m'(y :=\<^sub>s e)"
-  by (auto simp: upd_def st_upd_def intro!: state_rec.equality)
+(* lemma st_upd_eq [intro]: *)
+  (* "state_rec.more m = state_rec.more m' \<Longrightarrow>  *)
+              (* state_rec.cap m = state_rec.cap m' \<Longrightarrow> *)
+                 (* initState m = initState m' \<Longrightarrow> *)
+                    (* \<forall>x. x \<noteq> y \<longrightarrow> st m x = st m' x \<Longrightarrow> m(y :=\<^sub>s e) = m'(y :=\<^sub>s e)" *)
+  (* by (auto simp: upd_def st_upd_def intro!: state_rec.equality) *)
 
 
 
-lemma [simp]:
-  "rg (upd_part V f m) x = (if Reg x \<in> V then f (Reg x) else rg m x)"
-  unfolding rg_def upd_part_def
-  by simp
+(* lemma [simp]: *)
+  (* "rg (upd_part V f m) x = (if Reg x \<in> V then f (Reg x) else rg m x)" *)
+  (* unfolding  upd_part_def *)
+  (* by simp *)
 
-lemma [simp]:
-  "rg (m(aux: f)) = rg m"
-  unfolding rg_def aux_upd_def by simp
+(* lemma [simp]: *)
+  (* "rg (m(aux: f)) = rg m" *)
+  (* unfolding rg_def aux_upd_def by simp *)
 
 
 
 lemma eq_comm:
   "(a \<Longrightarrow> (b = c)) \<Longrightarrow> (a \<Longrightarrow> (c = b))" by blast
 
-
+(*
 
 lemma beh_substi [simp]:
   "st_beh\<^sub>i (subst\<^sub>i \<alpha> x e) = {(m\<^sub>1,upd_part (wr \<alpha>) (st m) m\<^sub>1) |m m\<^sub>1. (m\<^sub>1(x :=\<^sub>s st_ev\<^sub>E m\<^sub>1 e),m) \<in> st_beh\<^sub>i \<alpha>}"
@@ -266,6 +228,8 @@ lemma [simp]:
 lemma [simp]:
   "Base (st (m(x :=\<^sub>s e))) = Base ((st m)(x := Some e))"
   by (auto simp: st_upd_def)
+
+*)
 
 end (* of context expression *)
 end
