SimAsm/SimAsm.thy
@@ -2,15 +2,41 @@ theory SimAsm
   imports  "../Security"  SimAsm_Exp
 begin
 
+type_synonym ('s,'a) auxfn = "'s \<Rightarrow> 'a"
+type_synonym ('r,'v,'s,'a) auxop = "('r,'v) op \<times> ('s,'a) auxfn"
+
+type_synonym ('r,'v,'s,'a) opbasic = "(('r,'v,'s,'a) auxop, 's) basic"
+
+type_synonym ('r,'v,'s,'a) pred = "'s set"
+
+
+
+(* predicates are no longer sets of states but sets of trees, ie., of type predTree *)
+(* IF has another sub-command c\<^sub>3 to model the program after the If -- for the semantics of 
+         the speculation; even though for wp reasoning we make use of the wp(c\<^sub>3, Q) instead *)
+
+datatype ('r,'v,'s,'a) lang =
+  Skip
+  | Op "('r,'v,'s,'a) pred" "('r,'v) op" "('s,'a) auxfn"
+  | Seq "('r,'v,'s,'a) lang" "('r,'v,'s,'a) lang"
+  | If "('v,'r) bexp" "('r,'v,'s,'a) lang" "('r,'v,'s,'a) lang" "('r,'v,'s,'a) lang"  
+(*  | If "('v,'g,'r) bexp" "('r,'v,'s,'a) lang" "('r,'v,'s,'a) lang" *)
+  | While "('v,'r) bexp" "('r,'v,'s,'a) pred" "('r,'v,'s,'a) lang"
+  | DoWhile "('r,'v,'s,'a) pred" "('r,'v,'s,'a) lang" "('v,'r) bexp"
+
+
+context expression
+begin
+
 text \<open>Instruction Reordering\<close>
 text \<open>Only pattern match on first argument due to performance issues\<close>
-fun re\<^sub>i :: "('v,'g,'r) op \<Rightarrow> ('v,'g,'r) op \<Rightarrow> bool" 
+fun re\<^sub>i :: "('r,'v) op \<Rightarrow> ('r,'v) op \<Rightarrow> bool" 
   where
     "re\<^sub>i full_fence \<alpha> = False" |
     "re\<^sub>i (cmp b) \<alpha> = (\<alpha> \<noteq> full_fence \<and> wr \<alpha> \<subseteq> locals \<and> rd (cmp b) \<inter> wr \<alpha> = {} \<and> rd (cmp b) \<inter> rd \<alpha> \<subseteq> locals)" |
     "re\<^sub>i \<alpha> \<beta> = (\<beta> \<noteq> full_fence \<and> wr \<alpha> \<inter> wr \<beta> = {} \<and> rd \<alpha> \<inter> wr \<beta> = {} \<and> rd \<alpha> \<inter> rd \<beta> \<subseteq> locals)"
 
-fun re\<^sub>i' :: "('v,'g,'r) op \<Rightarrow> ('v,'g,'r) op \<Rightarrow> bool" where
+fun re\<^sub>i' :: "('r,'v) op \<Rightarrow> ('r,'v) op \<Rightarrow> bool" where
 "re\<^sub>i' full_fence \<alpha> = False" |
 "re\<^sub>i' \<alpha> full_fence = False" |
 "re\<^sub>i' (cmp b) \<alpha> = ((wr \<alpha> \<subseteq> locals) \<and> (wr \<alpha> \<inter> rd (cmp b) = {}) \<and> (rd (cmp b) \<inter> rd \<alpha> \<subseteq> locals))" |
@@ -19,7 +45,7 @@ fun re\<^sub>i' :: "('v,'g,'r) op \<Rightarrow> ('v,'g,'r) op \<Rightarrow> bool
 lemma "re\<^sub>i' \<alpha> \<beta> = re\<^sub>i \<alpha> \<beta>"
 by (induction rule: re\<^sub>i'.induct) auto
 
-fun fwd\<^sub>i  :: "('v,'g,'r) op \<Rightarrow> ('v,'g,'r) op \<Rightarrow> ('v,'g,'r) op" 
+fun fwd\<^sub>i  :: "('r,'v) op \<Rightarrow> ('r,'v) op \<Rightarrow> ('r,'v) op" 
   where "fwd\<^sub>i \<alpha> (assign x e) = subst\<^sub>i \<alpha> x e" | "fwd\<^sub>i \<alpha> _ = \<alpha>"
 
 section \<open>Auxiliary State Updates\<close>
@@ -31,12 +57,11 @@ This is achieved by allowing arbitrary extensions to the state representation, w
 can be updated atomically at any sub-operation.
 This auxiliary state cannot influence real execution behaviour by definition.
 \<close>
-type_synonym ('v,'g,'r,'a) auxop = "('v,'g,'r) op \<times> ('v,'g,'r,'a) auxfn"
 
-fun beh\<^sub>a :: "('v,'g,'r,'a) auxop \<Rightarrow> ('v,'g,'r,'a) state rel"
+fun beh\<^sub>a :: "('r,'v,'s,'a) auxop \<Rightarrow> 's rel"
   where "beh\<^sub>a (\<alpha>,f) = st_beh\<^sub>i \<alpha> O {(t,t'). t' = t(aux: f)}"
 
-fun re\<^sub>a :: "('v,'g,'r,'a) auxop \<Rightarrow> ('v,'g,'r,'a) auxop \<Rightarrow> bool" 
+fun re\<^sub>a :: "('r,'v,'s,'a) auxop \<Rightarrow> ('r,'v,'s,'a) auxop \<Rightarrow> bool" 
   where "re\<^sub>a (\<alpha>,_) (\<beta>,_) = re\<^sub>i \<alpha> \<beta>"
 
 
@@ -46,13 +71,12 @@ text \<open>
 To instantiate the abstract theory, we must couple each sub-operation with its precondition
 and behaviour in a tuple\<close>
 (* ('a,'b) basic = ('a \<times> 'b set \<times> 'b rel); 'a = (inst \<times> aux);  'b = state *)
-type_synonym ('v,'g,'r,'a) opbasic = "(('v,'g,'r,'a) auxop, ('v,'g,'r,'a) state) basic"
 
-fun re\<^sub>s :: "('v,'g,'r,'a) opbasic \<Rightarrow> ('v,'g,'r,'a) opbasic \<Rightarrow> bool"
+fun re\<^sub>s :: "('r,'v,'s,'a) opbasic \<Rightarrow> ('r,'v,'s,'a) opbasic \<Rightarrow> bool"
   where "re\<^sub>s (\<alpha>,_,_) (\<beta>,_,_) = re\<^sub>a \<alpha> \<beta>"
 
 text \<open>Duplicate forwarding and reordering behaviour of underlying instruction\<close>
-fun fwd\<^sub>s :: "('v,'g,'r,'a) opbasic \<Rightarrow> ('v,'g,'r,'a) auxop \<Rightarrow> ('v,'g,'r,'a) opbasic" 
+fun fwd\<^sub>s :: "('r,'v,'s,'a) opbasic \<Rightarrow> ('r,'v,'s,'a) auxop \<Rightarrow> ('r,'v,'s,'a) opbasic" 
   where 
     "fwd\<^sub>s ((\<alpha>,f),v,b) (assign x e,_) = (let p = (subst\<^sub>i \<alpha> x e, f) in  (p,v, beh\<^sub>a p))" |
     "fwd\<^sub>s ((\<alpha>,f),v,b) (leak c e,_) = ((\<alpha>,f),v,beh\<^sub>a (\<alpha>,f))" |
@@ -60,31 +84,21 @@ fun fwd\<^sub>s :: "('v,'g,'r,'a) opbasic \<Rightarrow> ('v,'g,'r,'a) auxop \<Ri
     "fwd\<^sub>s ((\<alpha>,f),v,b) (\<beta>,_) = ((\<alpha>,f),v,beh\<^sub>a (\<alpha>,f))"
 
 text \<open>Lift an operation with specification\<close>
-definition liftg :: "('v,'g,'r,'a) pred \<Rightarrow> ('v,'g,'r) op \<Rightarrow> ('v,'g,'r,'a) auxfn \<Rightarrow> ('v,'g,'r,'a) opbasic" 
+definition liftg :: "('r,'v,'s,'a) pred \<Rightarrow> ('r,'v) op \<Rightarrow> ('s,'a) auxfn \<Rightarrow> ('r,'v,'s,'a) opbasic" 
   ("\<lfloor>_,_,_\<rfloor>" 100)
   where "liftg v \<alpha> f \<equiv> ((\<alpha>,f), v, beh\<^sub>a (\<alpha>,f))"
 
 text \<open>Lift an operation without specification\<close>
-definition liftl :: "('v,'g,'r) op \<Rightarrow> ('v,'g,'r,'a) opbasic" 
+definition liftl :: "('r,'v) op \<Rightarrow> ('r,'v,'s,'a) opbasic" 
   ("\<lfloor>_\<rfloor>" 100)
-  where "liftl \<alpha> \<equiv> ((\<alpha>,state_rec.more), UNIV, beh\<^sub>a (\<alpha>,state_rec.more))"
+  where "liftl \<alpha> \<equiv> ((\<alpha>,aux), UNIV, beh\<^sub>a (\<alpha>,aux))"
 
 section \<open>Language Definition\<close>
 
 
-(* predicates are no longer sets of states but sets of trees, ie., of type predTree *)
-(* IF has another sub-command c\<^sub>3 to model the program after the If -- for the semantics of 
-         the speculation; even though for wp reasoning we make use of the wp(c\<^sub>3, Q) instead *)
-
-datatype ('v,'g,'r,'a) lang =
-  Skip
-  | Op "('v,'g,'r,'a) pred" "('v,'g,'r) op" "('v,'g,'r,'a) auxfn"
-  | Seq "('v,'g,'r,'a) lang" "('v,'g,'r,'a) lang"
-  | If "('v,'g,'r) bexp" "('v,'g,'r,'a) lang" "('v,'g,'r,'a) lang" "('v,'g,'r,'a) lang"  
-(*  | If "('v,'g,'r) bexp" "('v,'g,'r,'a) lang" "('v,'g,'r,'a) lang" *)
-  | While "('v,'g,'r) bexp" "('v,'g,'r,'a) pred" "('v,'g,'r,'a) lang"
-  | DoWhile "('v,'g,'r,'a) pred" "('v,'g,'r,'a) lang" "('v,'g,'r) bexp"
 
 
+
+end
 
 end
